functional-programming-lean/src/type-classes.md
@@ -1,13 +1,13 @@
 # Overloading and Type Classes
 
 In many languages, the built-in datatypes get special treatment.
-For instance, in C and Java, `+` can be used to add `float`s and `int`s, but not arbitrary-precision numbers from a third-party library.
+For example, in C and Java, `+` can be used to add `float`s and `int`s, but not arbitrary-precision numbers from a third-party library.
 Similarly, numeric literals can be used directly for the built-in types, but not for user-defined number types.
 Other languages provide an _overloading_ mechanism for operators, where the same operator can be given a meaning for a new type.
 In these languages, such as C++ and C#, a wide variety of built-in operators can be overloaded, and the compiler uses the type checker to select a particular implementation.
 
 In addition to numeric literals and operators, many languages allow overloading of functions or methods.
-For instance, in C++, Java, C# and Kotlin, multiple implementations of a method are allowed, with differing numbers and types of arguments.
+In C++, Java, C# and Kotlin, multiple implementations of a method are allowed, with differing numbers and types of arguments.
 The compiler uses the number of arguments and their types to determine which overload was intended.
 
 Function and operator overloading has a key limitation: polymorphic functions can't restrict their type arguments to types for which a given overload exists.
@@ -19,7 +19,7 @@ If programmers are not very careful, this can lead to programs that crash at run
 Lean implements overloading using a mechanism called _type classes_, pioneered in Haskell, that allows overloading of operators, functions, and literals in a manner that works well with polymorphism.
 A type class describes a collection of overloadable operations.
 To overload these operations for a new type, an _instance_ is created that contains an implementation of each operation for the new type.
-For instance, a type class named `Add` describes types that allow addition, and an instance of `Add` for `Nat` provides an implementation of addition for `Nat`.
+For example, a type class named `Add` describes types that allow addition, and an instance of `Add` for `Nat` provides an implementation of addition for `Nat`.
 
 The terms _class_ and _instance_ can be confusing for those who are used to object-oriented languages, because they are not closely related to classes and instances in object-oriented languages.
 However, they do share common roots: in everyday language, the term "class" refers to a group that shares some common attributes.
