functional-programming-lean/src/type-classes/standard-classes.md
@@ -1,7 +1,8 @@
 # Standard Classes
 
-This section presents a variety of operators that can be overloaded using type classes in Lean.
-After skimming it to see what's available, it's probably most useful as a reference later on.
+This section presents a variety of operators and functions that can be overloaded using type classes in Lean.
+Each operator or function corresponds to a method of a type class.
+Unlike C++, infix operators in Lean are defined as abbreviations for named functions; this means that overloading them for new types is not done using the operator itself, but rather refers to a name such as `HAdd.hAdd`.
 
 ## Arithmetic
 
@@ -11,12 +12,12 @@ The following arithmetic operators are overloaded:
 
 | Expression | Desugaring | Class Name |
 |------------|------------|------------|
-| `{{#example_in Examples/Classes.lean plusDesugar}}` | `{{#example_out Examples/Classes.lean plusDesugar}}` | `Add` |
-| `{{#example_in Examples/Classes.lean minusDesugar}}` | `{{#example_out Examples/Classes.lean minusDesugar}}` | `Sub` |
-| `{{#example_in Examples/Classes.lean timesDesugar}}` | `{{#example_out Examples/Classes.lean timesDesugar}}` | `Mul` |
-| `{{#example_in Examples/Classes.lean divDesugar}}` | `{{#example_out Examples/Classes.lean divDesugar}}` | `Div` |
-| `{{#example_in Examples/Classes.lean modDesugar}}` | `{{#example_out Examples/Classes.lean modDesugar}}` | `Mod` |
-| `{{#example_in Examples/Classes.lean powDesugar}}` | `{{#example_out Examples/Classes.lean powDesugar}}` | `Pow` |
+| `{{#example_in Examples/Classes.lean plusDesugar}}` | `{{#example_out Examples/Classes.lean plusDesugar}}` | `HAdd` |
+| `{{#example_in Examples/Classes.lean minusDesugar}}` | `{{#example_out Examples/Classes.lean minusDesugar}}` | `HSub` |
+| `{{#example_in Examples/Classes.lean timesDesugar}}` | `{{#example_out Examples/Classes.lean timesDesugar}}` | `HMul` |
+| `{{#example_in Examples/Classes.lean divDesugar}}` | `{{#example_out Examples/Classes.lean divDesugar}}` | `HDiv` |
+| `{{#example_in Examples/Classes.lean modDesugar}}` | `{{#example_out Examples/Classes.lean modDesugar}}` | `HMod` |
+| `{{#example_in Examples/Classes.lean powDesugar}}` | `{{#example_out Examples/Classes.lean powDesugar}}` | `HPow` |
 | `{{#example_in Examples/Classes.lean negDesugar}}` | `{{#example_out Examples/Classes.lean negDesugar}}` | `Neg` |
 
 
@@ -29,12 +30,14 @@ The following bitwise operators are overloaded:
 
 | Expression | Desugaring | Class Name |
 |------------|------------|------------|
-| `{{#example_in Examples/Classes.lean bAndDesugar}}` | `{{#example_out Examples/Classes.lean bAndDesugar}}` | `AndOp` |
-| <code class="hljs">x &#x7c;&#x7c;&#x7c; y </code> | `{{#example_out Examples/Classes.lean bOrDesugar}}` | `OrOp` |
-| `{{#example_in Examples/Classes.lean bXorDesugar}}` | `{{#example_out Examples/Classes.lean bXorDesugar}}` | `Xor` |
+| `{{#example_in Examples/Classes.lean bAndDesugar}}` | `{{#example_out Examples/Classes.lean bAndDesugar}}` | `HAnd` |
+| <code class="hljs">x &#x7c;&#x7c;&#x7c; y </code> | `{{#example_out Examples/Classes.lean bOrDesugar}}` | `HOr` |
+| `{{#example_in Examples/Classes.lean bXorDesugar}}` | `{{#example_out Examples/Classes.lean bXorDesugar}}` | `HXor` |
 | `{{#example_in Examples/Classes.lean complementDesugar}}` | `{{#example_out Examples/Classes.lean complementDesugar}}` | `Complement` |
-| `{{#example_in Examples/Classes.lean shrDesugar}}` | `{{#example_out Examples/Classes.lean shrDesugar}}` | `ShiftRight` |
-| `{{#example_in Examples/Classes.lean shlDesugar}}` | `{{#example_out Examples/Classes.lean shlDesugar}}` | `ShiftLeft` |
+| `{{#example_in Examples/Classes.lean shrDesugar}}` | `{{#example_out Examples/Classes.lean shrDesugar}}` | `HShiftRight` |
+| `{{#example_in Examples/Classes.lean shlDesugar}}` | `{{#example_out Examples/Classes.lean shlDesugar}}` | `HShiftLeft` |
+
+Because the names `And` and `Or` are already taken as the names of logical connectives, the homogeneous versions of `HAnd` and `HOr` are called `AndOp` and `OrOp` rather than `And` and `Or`.
 
 ## Equality and Ordering
 
@@ -45,10 +48,10 @@ Due to Lean's use as a theorem prover, there are really two kinds of equality op
  
 Both notions of equality are important, and used for different purposes.
 Boolean equality is useful in programs, when a decision needs to be made about whether two values are equal.
-For instance, `{{#example_in Examples/Classes.lean boolEqTrue}}` evaluates to `{{#example_out Examples/Classes.lean boolEqTrue}}`, and `{{#example_in Examples/Classes.lean boolEqFalse}}` evaluates to `{{#example_out Examples/Classes.lean boolEqFalse}}`.
+For example, `{{#example_in Examples/Classes.lean boolEqTrue}}` evaluates to `{{#example_out Examples/Classes.lean boolEqTrue}}`, and `{{#example_in Examples/Classes.lean boolEqFalse}}` evaluates to `{{#example_out Examples/Classes.lean boolEqFalse}}`.
 Some values, such as functions, cannot be checked for equality.
 For example, `{{#example_in Examples/Classes.lean functionEq}}` yields the error:
-```Lean error
+```output error
 {{#example_out Examples/Classes.lean functionEq}}
 ```
 As this message indicates, `==` is overloaded using a type class.
@@ -67,24 +70,24 @@ Some propositions are _decidable_, which means that they can be checked just lik
 The function that checks whether the proposition is true or false is called a _decision procedure_, and it returns _evidence_ of the truth or falsity of the proposition.
 Some examples of decidable propositions include equality and inequality of natural numbers, equality of strings, and "ands" and "ors" of propositions that are themselves decidable.
 
-In Lean, decidable propositions can be used just like Booleans.
+In Lean, `if` works with decidable propositions.
 For example, `2 < 4` is a proposition:
-```Lean
+```lean
 {{#example_in Examples/Classes.lean twoLessFour}}
 ```
-```Lean info
+```output info
 {{#example_out Examples/Classes.lean twoLessFour}}
 ```
 Nonetheless, it is perfectly acceptable to write it as the condition in an `if`.
-For instance, `{{#example_in Examples/Classes.lean ifProp}}` has type `Nat` and evaluates to `{{#example_out Examples/Classes.lean ifProp}}`.
+For example, `{{#example_in Examples/Classes.lean ifProp}}` has type `Nat` and evaluates to `{{#example_out Examples/Classes.lean ifProp}}`.
 
 
 Not all propositions are decidable.
-If they were, then computers would be able to prove any true proposition just by running the decision procedure.
+If they were, then computers would be able to prove any true proposition just by running the decision procedure, and mathematicians would be out of a job.
 More specifically, decidable propositions have an instance of the `Decidable` type class which has a method that is the decision procedure.
 Trying to use a proposition that isn't decidable as if it were a `Bool` results in a failure to find the `Decidable` instance.
 For example, `{{#example_in Examples/Classes.lean funEqDec}}` results in:
-```Lean error
+```output error
 {{#example_out Examples/Classes.lean funEqDec}}
 ```
 
@@ -96,6 +99,7 @@ The following propositions, that are usually decidable, are overloaded with type
 | `{{#example_in Examples/Classes.lean leDesugar}}` | `{{#example_out Examples/Classes.lean leDesugar}}` | `LE` |
 | `{{#example_in Examples/Classes.lean gtDesugar}}` | `{{#example_out Examples/Classes.lean gtDesugar}}` | `LT` |
 | `{{#example_in Examples/Classes.lean geDesugar}}` | `{{#example_out Examples/Classes.lean geDesugar}}` | `LE` |
+
 Because defining new propositions hasn't yet been demonstrated, it may be difficult to define new instances of `LT` and `LE`.
 
 Additionally, comparing values using `<`, `==`, and `>` can be inefficient.
@@ -103,12 +107,12 @@ Checking first whether one value is less than another, and then whether they are
 To solve this problem, Java and C# have standard `compareTo` and `CompareTo` methods (respectively) that can be overridden by a class in order to implement all three operations at the same time.
 These methods return a negative integer if the receiver is less than the argument, zero if they are equal, and a positive integer if the receiver is greater than the argument.
 Rather than overload the meaning of integers, Lean has a built-in inductive type that describes these three possibilities:
-```Lean
+```lean
 {{#example_decl Examples/Classes.lean Ordering}}
 ```
 The `Ord` type class can be overloaded to produce these comparisons.
 For `Pos`, an implementation can be:
-```Lean
+```lean
 {{#example_decl Examples/Classes.lean OrdPos}}
 ```
 In situations where `compareTo` would be the right approach in Java, use `Ord.compare` in Lean.
@@ -117,25 +121,30 @@ In situations where `compareTo` would be the right approach in Java, use `Ord.co
 
 Java and C# have `hashCode` and `GetHashCode` methods, respectively, that compute a hash of a value for use in data structures such as hash tables.
 The Lean equivalent is a type class called `Hashable`:
-```Lean
+```lean
 {{#example_decl Examples/Classes.lean Hashable}}
 ```
 If two values are considered equal according to a `BEq` instance for their type, then they should have the same hashes.
 In other words, if `x == y` then `hash x == hash y`.
-If `x != y`, then `hash x` won't necessarily differ from `hash y` (after all, there are infinitely more `Nat` values than there are `UInt64` values), but data structures built on hashing will have better performance if unequal values are likely to have unequal hashes.
+If `x ≠ y`, then `hash x` won't necessarily differ from `hash y` (after all, there are infinitely more `Nat` values than there are `UInt64` values), but data structures built on hashing will have better performance if unequal values are likely to have unequal hashes.
 This is the same expectation as in Java and C#.
 
 The standard library contains a function `{{#example_in Examples/Classes.lean mixHash}}` with type `{{#example_out Examples/Classes.lean mixHash}}` that can be used to combine hashes for different fields for a constructor.
 A reasonable hash function for an inductive datatype can be written by assigning a unique number to each constructor, and then mixing that number with the hashes of each field.
-For instance, a `Hashable` instance for `Pos` can be written:
-```Lean
+For example, a `Hashable` instance for `Pos` can be written:
+```lean
 {{#example_decl Examples/Classes.lean HashablePos}}
 ```
 `Hashable` instances for polymorphic types can use recursive instance search.
-For instance, hashing a `NonEmptyList α` is only possible when `α` can be hashed:
-```Lean
+Hashing a `NonEmptyList α` is only possible when `α` can be hashed:
+```lean
 {{#example_decl Examples/Classes.lean HashableNonEmptyList}}
 ```
+Binary trees use both recursion and recursive instance search in the implementations of `BEq` and `Hashable`:
+```lean
+{{#example_decl Examples/Classes.lean TreeHash}}
+```
+
 
 ## Deriving Standard Classes
 
@@ -150,7 +159,7 @@ For a type that is already defined, a standalone `deriving` command can be used.
 Write `deriving instance C1, C2, ... for T` to deriving instances of `C1, C2, ...` for the type `T` after the fact.
 
 `BEq` and `Hashable` instances can be derived for `Pos` and `NonEmptyList` using a very small amount of code:
-```Lean
+```lean
 {{#example_decl Examples/Classes.lean BEqHashableDerive}}
 ```
 
@@ -160,45 +169,46 @@ Instance can be derived for at least the following classes:
  * `Repr`
  * `Hashable`
  * `Ord`
+
 In some cases, however, the derived `Ord` instance may not produce precisely the ordering desired in an application.
 When this is the case, it's fine to write an `Ord` instance by hand.
 The collection of classes for which instances can be derived can be extended by advanced users of Lean.
 
 Aside from the clear advantages in programmer productivity and code readability, deriving instances also makes code easier to maintain, because the instances are updated as the definitions of types evolve.
-Changesets involving updates to datatypes need not also have line after line of formulaic modifications to equality tests and hash computation.
+Changesets involving updates to datatypes are easier to read without line after line of formulaic modifications to equality tests and hash computation.
 
 ## Appending
 
 Many datatypes have some sort of append operator.
 In Lean, appending two values is overloaded with the type class `HAppend`, which is a heterogeneous operation like that used for arithmetic operations:
-```Lean
+```lean
 {{#example_decl Examples/Classes.lean HAppend}}
 ```
 The syntax `{{#example_in Examples/Classes.lean desugarHAppend}}` desugars to `{{#example_out Examples/Classes.lean desugarHAppend}}`.
 For homogeneous cases, it's enough to implement an instance of `Append`, which follows the usual pattern:
-```Lean
+```lean
 {{#example_decl Examples/Classes.lean AppendNEList}}
 ```
 
 After defining the above instance,
-```Lean
+```lean
 {{#example_in Examples/Classes.lean appendSpiders}}
 ```
 has the following output:
-```Lean info
+```output info
 {{#example_out Examples/Classes.lean appendSpiders}}
 ```
 
 Similarly, a definition of `HAppend` allows non-empty lists to be appended to ordinary lists:
-```Lean
+```lean
 {{#example_decl Examples/Classes.lean AppendNEListList}}
 ```
 With this instance available,
-```Lean
+```lean
 {{#example_in Examples/Classes.lean appendSpidersList}}
 ```
 results in
-```Lean info
+```output info
 {{#example_out Examples/Classes.lean appendSpidersList}}
 ```
 
@@ -221,7 +231,7 @@ The prior examples can be rewritten as follows:
  * `{{#example_in Examples/Classes.lean mapInfixListList}}` evaluates to `{{#example_out Examples/Classes.lean mapInfixListList}}`
 
 An instance of `Functor` for `NonEmptyList` requires specifying the `map` function.
-```Lean
+```lean
 {{#example_decl Examples/Classes.lean FunctorNonEmptyList}}
 ```
 Here, `map` uses the `Functor` instance for `List` to map the function over the tail.
@@ -230,7 +240,7 @@ A `NonEmptyList` can have a function mapped over it _no matter what the type of 
 If `α` were a parameter to the class, then it would be possible to make versions of `Functor` that only worked for `NonEmptyList Nat`, but part of being a functor is that `map` works for any entry type.
 
 Here is an instance of `Functor` for `PPoint`:
-```Lean
+```lean
 {{#example_decl Examples/Classes.lean FunctorPPoint}}
 ```
 In this case, `f` has been applied to both `x` and `y`.
@@ -240,8 +250,8 @@ That is, when using `map` on a `NonEmptyList (PPoint Nat)`, the function being m
 
 The definition of the `Functor` class uses one more language feature that has not yet been discussed: default method definitions.
 Normally, a class will specify some minimal set of overloadable operations that make sense together, and then use polymorphic functions with instance implicit arguments that build on the overloaded operations to provide a larger library of features.
-For instance, the function `concat` can concatenate any non-empty list whose entries are appendable:
-```Lean
+For example, the function `concat` can concatenate any non-empty list whose entries are appendable:
+```lean
 {{#example_decl Examples/Classes.lean concat}}
 ```
 However, for some classes, there are operations that can be more efficiently implemented with knowledge of the internals of a datatype.
@@ -253,13 +263,13 @@ Default method definitions contain `:=` in a `class` definition.
 
 In the case of `Functor`, some types have a more efficient way of implementing `map` when the function being mapped ignores its argument.
 Functions that ignore their arguments are called _constant functions_ because they always return the same value.
-Here is the definition of `Functor`:
-```Lean
+Here is the definition of `Functor`, in which `mapConst` has a default implementation:
+```lean
 {{#example_decl Examples/Classes.lean FunctorDef}}
 ```
 
 Just as a `Hashable` instance that doesn't respect `BEq` is buggy, a `Functor` instance that moves around the data as it maps the function is also buggy.
-For instance, a buggy `Functor` instance for `List` might throw away its argument and always return the empty list, or it might reverse the list.
+For example, a buggy `Functor` instance for `List` might throw away its argument and always return the empty list, or it might reverse the list.
 A bad instance for `PPoint` might place `f x` in both the `x` and the `y` fields.
 Specifically, `Functor` instances should follow two rules:
  1. Mapping the identity function should result in the original argument.
@@ -273,4 +283,4 @@ These rules prevent implementations of `map` that move the data around or delete
 ## Exercises
 
  * Write an instance of `HAppend (List α) (NonEmptyList α) (NonEmptyList α)` and test it.
- * Define a datatype that represents binary trees. Implement a `Functor` instance for this datatype.
+ * Implement a `Functor` instance for the binary tree datatype.
